verify that all sorted list theorems don't depend on axioms except propext

Root2/SortedList.lean
@@ -5,15 +5,21 @@ def contains (as: List α) (a: α) : Prop := match as with
   | [] => False
   | x :: xs => a = x ∨ contains xs a
 
+#print axioms List.contains
+
 @[simp]
 def List.allP  (list: List a) (P : a -> Prop) : Prop := match list with
   | [] => True
   | x :: xs => P x ∧ allP xs P
 
+#print axioms List.allP
+
 @[simp]
 def List.anyP (list: List a) (P : a -> Prop) : Prop := match list with
   | [] => False
   | x :: xs => P x ∨ anyP xs P
+
+#print axioms List.anyP
 
 @[simp]
 def List.mapAllP {{list: List a}} {{ P R: a -> Prop }} (all: list.allP P) (F: ∀a, P a -> R a) : list.allP R := by
@@ -25,6 +31,8 @@ def List.mapAllP {{list: List a}} {{ P R: a -> Prop }} (all: list.allP P) (F: �
     exact F x all.left
     exact List.mapAllP all.right F
 
+#print axioms List.mapAllP
+
 @[simp]
 def List.mapAnyP {{list: List a}} {{ P R: a -> Prop }} (any: list.anyP P) (F: ∀a, P a -> R a) : list.anyP R := by
   match list with
@@ -34,6 +42,8 @@ def List.mapAnyP {{list: List a}} {{ P R: a -> Prop }} (any: list.anyP P) (F: �
     match any with
     | .inl prf => exact .inl (F x prf)
     | .inr prf => exact .inr (List.mapAnyP prf F)
+
+#print axioms List.mapAnyP
 
 @[simp]
 def List.any_and_not_all {{list: List a}} {{ P: a -> Prop }} (not_all: list.allP fun x => ¬ P x) (any: list.anyP P) : False := by
@@ -48,6 +58,8 @@ def List.any_and_not_all {{list: List a}} {{ P: a -> Prop }} (not_all: list.allP
     | .inr prf => 
       apply any_and_not_all not_all.right prf
 
+#print axioms List.any_and_not_all
+
 @[simp]
 def List.all_and_not_all {{list: List a}} {{ P: a -> Prop }} (not_all: list.allP fun x => ¬ P x) (all: list.allP P) : list = [] := by
   match list with
@@ -58,15 +70,21 @@ def List.all_and_not_all {{list: List a}} {{ P: a -> Prop }} (not_all: list.allP
     have p := all.left
     contradiction
 
+#print axioms List.all_and_not_all
+
 @[simp]
 def List.sorted_by (list: List a) (P : a -> a -> Prop) : Prop := match list with
   | [] | [_] => True
   | a :: b :: xs => P a b ∧ sorted_by (b :: xs) P
 
+#print axioms List.sorted_by
+
 @[simp]
 def List.sorted [Compare α] (list: List α) : Prop := match list with
   | [] | [_] => True
   | a :: b :: xs => b <= a ∧ sorted (b :: xs)
+
+#print axioms List.sorted
 
 @[simp]
 def List.concat_sorted [Compare α] (a b: List α) : List α := match a with
@@ -102,8 +120,10 @@ decreasing_by {
   }
 }
 
+#print axioms List.concat_sorted
+
 @[simp]
-def List.concat_sorted.induction [Compare α]
+def concat_sorted.induction [Compare α]
   {P: List α -> List α -> Prop}
   (empty_left: ∀ bs, P [] bs)
   (empty_right: ∀ a as, P (a::as) [])
@@ -117,12 +137,12 @@ def List.concat_sorted.induction [Compare α]
 | [] => empty_right a as
 | b::bs => match h:Compare.ord a b with
 | .Eq =>
-  induct_eq a b as bs (Compare.ord_implies_eq h) (List.concat_sorted.induction empty_left empty_right induct_lt induct_eq induct_gt as bs)
+  induct_eq a b as bs (Compare.ord_implies_eq h) (concat_sorted.induction empty_left empty_right induct_lt induct_eq induct_gt as bs)
 | .Less =>
-  induct_lt a b as bs h (List.concat_sorted.induction empty_left empty_right induct_lt induct_eq induct_gt (a::as) bs)
+  induct_lt a b as bs h (concat_sorted.induction empty_left empty_right induct_lt induct_eq induct_gt (a::as) bs)
 | .Greater =>
-  induct_gt a b as bs (Compare.flip h) (List.concat_sorted.induction empty_left empty_right induct_lt induct_eq induct_gt as (b::bs))
-termination_by List.concat_sorted.induction a b => a.length + b.length
+  induct_gt a b as bs (Compare.flip h) (concat_sorted.induction empty_left empty_right induct_lt induct_eq induct_gt as (b::bs))
+termination_by concat_sorted.induction a b => a.length + b.length
 decreasing_by {
   simp_wf
   try {
@@ -139,227 +159,248 @@ decreasing_by {
   }
 }
 
-section concat_sorted
-  theorem empty_left [Compare α] {{as: List α}} : List.concat_sorted as [] = as := by
-    cases as <;> simp
+#print axioms concat_sorted.induction
 
-  theorem empty_right [Compare α] {{as: List α}} : List.concat_sorted [] as = as := by
-    cases as <;> simp
+theorem concat_sorted.empty_left [Compare α] {{as: List α}} : List.concat_sorted as [] = as := by
+  cases as <;> simp
 
-  theorem pop [Compare α] {{a: α}} {{as: List α}} : (a::as).sorted -> as.sorted := by
-    intro list_sorted
+#print axioms concat_sorted.empty_left
+
+theorem concat_sorted.empty_right [Compare α] {{as: List α}} : List.concat_sorted [] as = as := by
+  cases as <;> simp
+
+#print axioms concat_sorted.empty_right
+
+theorem concat_sorted.pop [Compare α] {{a: α}} {{as: List α}} : (a::as).sorted -> as.sorted := by
+  intro list_sorted
+  match as with
+  | [] => trivial
+  | a₀::as₀ => exact list_sorted.right
+
+#print axioms concat_sorted.pop
+
+theorem concat_sorted.singleton_list_is_sorted [Compare α] {a: α} : [a].sorted := by simp
+
+#print axioms concat_sorted.singleton_list_is_sorted
+
+theorem concat_sorted.take_fst [Compare α] {{ a b : α }} (b_lt_a: b < a) :
+  a :: (List.concat_sorted as (b::bs)) = List.concat_sorted (a::as) (b::bs) := by
+  simp
+  have : Compare.ord a b = Order.Greater := Compare.flip b_lt_a
+  rw [this]
+
+#print axioms concat_sorted.take_fst
+
+theorem concat_sorted.take_snd [Compare α] {{ a b : α }} (a_lt_b: a < b) :
+  b :: (List.concat_sorted (a::as) bs) = List.concat_sorted (a::as) (b::bs)  := by
+  simp
+  rw [a_lt_b]
+
+#print axioms concat_sorted.take_snd
+
+theorem concat_sorted.list_sorted_fst_snd_empty [Compare α] {{ a : α }} (aas_sorted : (a :: as).sorted) :
+  List.sorted (a :: List.concat_sorted as []) := by
+  rw [empty_left]
+  assumption
+
+#print axioms concat_sorted.list_sorted_fst_snd_empty
+
+theorem concat_sorted.list_sorted_snd_fst_empty [Compare α] {{ a : α }} (bbs_sorted : (a :: as).sorted) :
+  List.sorted (a :: List.concat_sorted [] as) := by
+  rw [empty_right]
+  assumption
+
+#print axioms concat_sorted.list_sorted_snd_fst_empty
+
+theorem concat_sorted.list_sorted_nonempty [Compare α] {{ a b: α }} (as bs : List α)
+    (aas: (a::as).sorted) (bbs : (b::bs).sorted)
+  :
+    (b <= a -> List.sorted (a::List.concat_sorted as (b::bs)))
+    ∧ 
+    (a <= b -> List.sorted (b::List.concat_sorted (a::as) bs)) := by
     match as with
-    | [] => trivial
-    | a₀::as₀ => exact list_sorted.right
-
-  theorem singleton_list_is_sorted [Compare α] {a: α} : [a].sorted := by simp
-
-  theorem take_fst [Compare α] {{ a b : α }} (b_lt_a: b < a) :
-    a :: (List.concat_sorted as (b::bs)) = List.concat_sorted (a::as) (b::bs) := by
-    simp
-    have : Compare.ord a b = Order.Greater := Compare.flip b_lt_a
-    rw [this]
-
-  theorem take_snd [Compare α] {{ a b : α }} (a_lt_b: a < b) :
-    b :: (List.concat_sorted (a::as) bs) = List.concat_sorted (a::as) (b::bs)  := by
-    simp
-    rw [a_lt_b]
-
-  theorem list_sorted_fst_snd_empty [Compare α] {{ a : α }} (aas_sorted : (a :: as).sorted) :
-    List.sorted (a :: List.concat_sorted as []) := by
-    rw [empty_left]
-    assumption
-
-  theorem list_sorted_snd_fst_empty [Compare α] {{ a : α }} (bbs_sorted : (a :: as).sorted) :
-    List.sorted (a :: List.concat_sorted [] as) := by
-    rw [empty_right]
-    assumption
-
-  theorem list_sorted_nonempty [Compare α] {{ a b: α }} (as bs : List α)
-      (aas: (a::as).sorted) (bbs : (b::bs).sorted)
-    :
-      (b <= a -> List.sorted (a::List.concat_sorted as (b::bs)))
-      ∧ 
-      (a <= b -> List.sorted (b::List.concat_sorted (a::as) bs)) := by
-      match as with
-      | [] =>
-        rw [empty_right]
+    | [] =>
+      rw [empty_right]
+      apply And.intro
+      {
+        intro b_le_a
         apply And.intro
-        {
-          intro b_le_a
-          apply And.intro
-          assumption
-          assumption
-        }
-        {
-          intro a_le_b
-          match bs with
-          | [] =>
-            rw [empty_left]
-            apply And.intro <;>
-            assumption
-          | b'::bs' =>
-            have :  List.length bs' < Nat.succ (List.length bs') := Nat.lt_succ_self _
-            have ⟨ _, right ⟩  := @list_sorted_nonempty α _ a b' [] bs' aas bbs.right
-            unfold List.concat_sorted
-            simp only
-            cases h:Compare.ord a b' <;> simp
-            apply And.intro
-            exact bbs.left
-            exact right (Or.inl h)
-            apply And.intro
-            exact a_le_b
-            apply And.intro
-            exact (Or.inr (Compare.flip h))
-            exact bbs.right
-            apply And.intro
-            exact a_le_b
-            apply And.intro
-            exact (Or.inl (Compare.flip h))
-            exact bbs.right
-        }
-      | a'::as' => 
+        assumption
+        assumption
+      }
+      {
+        intro a_le_b
         match bs with
         | [] =>
           rw [empty_left]
+          apply And.intro <;>
+          assumption
+        | b'::bs' =>
+          have :  List.length bs' < Nat.succ (List.length bs') := Nat.lt_succ_self _
+          have ⟨ _, right ⟩  := @list_sorted_nonempty α _ a b' [] bs' aas bbs.right
+          unfold List.concat_sorted
+          simp only
+          cases h:Compare.ord a b' <;> simp
           apply And.intro
+          exact bbs.left
+          exact right (Or.inl h)
+          apply And.intro
+          exact a_le_b
+          apply And.intro
+          exact (Or.inr (Compare.flip h))
+          exact bbs.right
+          apply And.intro
+          exact a_le_b
+          apply And.intro
+          exact (Or.inl (Compare.flip h))
+          exact bbs.right
+      }
+    | a'::as' => 
+      match bs with
+      | [] =>
+        rw [empty_left]
+        apply And.intro
+        {
+          intro b_le_a
+          unfold List.concat_sorted
+          simp only
+          cases h:Compare.ord a' b <;> simp
+          apply And.intro
+          exact b_le_a
+          apply And.intro
+          exact Or.inl h
+          exact aas.right
+          apply And.intro
+          exact aas.left
+          apply And.intro
+          exact (Or.inr (Compare.flip h))
+          rw [empty_left]
+          have : a' = b := Compare.ord_implies_eq h 
+          rw [← this]
+          exact aas.right
+          apply And.intro
+          exact aas.left
+          have : List.length as' < List.length as' + 1 := Nat.lt_succ_self _
+          have ⟨ left, _ ⟩  := @list_sorted_nonempty α _ a' b as' [] aas.right bbs
+          exact left (Or.inl (Compare.flip h))
+        }
+        {
+          intro a_le_b
+          apply And.intro
+          exact a_le_b
+          exact aas
+        }
+      | b'::bs' =>
+        simp only
+        apply And.intro
+        {
+          unfold List.concat_sorted
+          intro b_le_a
+          simp only
+          cases h₀:Compare.ord a' b
           {
-            intro b_le_a
-            unfold List.concat_sorted
-            simp only
-            cases h:Compare.ord a' b <;> simp
             apply And.intro
             exact b_le_a
-            apply And.intro
-            exact Or.inl h
-            exact aas.right
-            apply And.intro
-            exact aas.left
-            apply And.intro
-            exact (Or.inr (Compare.flip h))
-            rw [empty_left]
-            have : a' = b := Compare.ord_implies_eq h 
-            rw [← this]
-            exact aas.right
-            apply And.intro
-            exact aas.left
-            have : List.length as' < List.length as' + 1 := Nat.lt_succ_self _
-            have ⟨ left, _ ⟩  := @list_sorted_nonempty α _ a' b as' [] aas.right bbs
-            exact left (Or.inl (Compare.flip h))
+            have : List.length as' + Nat.succ (List.length bs') < Nat.succ (List.length as') + Nat.succ (List.length bs') := by
+              apply Nat.add_lt_add_right
+              apply Nat.lt_succ_self
+            have ⟨ _, right ⟩  := @list_sorted_nonempty α _ a' b as' (b'::bs') aas.right bbs
+            exact right (Or.inl h₀)
           }
           {
-            intro a_le_b
+            apply And.intro
+            exact aas.left
+            apply And.intro
+            exact Or.inr (Compare.flip h₀)
+            match as' with
+            | [] =>
+              rw [empty_right]
+              exact bbs
+            | a''::as'' =>
+              have : List.length as'' + Nat.succ (List.length bs') < Nat.succ (Nat.succ (List.length as'')) + Nat.succ (List.length bs') := by
+                apply Nat.add_lt_add_right
+                apply Nat.lt_trans (Nat.lt_succ_self _)
+                apply Nat.lt_succ_self
+              have ⟨ _, right ⟩  := @list_sorted_nonempty α _ a'' b as'' (b'::bs') aas.right.right bbs
+              apply right
+              have : a' = b := Compare.ord_implies_eq h₀
+              rw [←this]
+              exact aas.right.left
+          }
+          {
+            apply And.intro
+            exact aas.left
+            have : List.length as' + Nat.succ (List.length bs') < Nat.succ (List.length as') + Nat.succ (List.length bs') := by
+              apply Nat.add_lt_add_right
+              apply Nat.lt_succ_self
+            have ⟨ left, _ ⟩  := @list_sorted_nonempty α _ a' b as' (b'::bs') aas.right bbs
+            exact left (Or.inl (Compare.flip h₀))
+          }
+        }
+        {
+          unfold List.concat_sorted
+          intro a_le_b
+          simp only
+          cases h₀:Compare.ord a b'
+          {
+            apply And.intro
+            exact bbs.left
+            have : Nat.succ (List.length as') + List.length bs' < Nat.succ (List.length as') + Nat.succ (List.length bs') := by
+              apply Nat.add_lt_add_left
+              apply Nat.lt_succ_self
+            have ⟨ _, right ⟩  := @list_sorted_nonempty α _ a b' (a'::as') bs' aas bbs.right
+            exact right (Or.inl h₀)
+          }
+          {
             apply And.intro
             exact a_le_b
-            exact aas
-          }
-        | b'::bs' =>
-          simp only
-          apply And.intro
-          {
-            unfold List.concat_sorted
-            intro b_le_a
-            simp only
-            cases h₀:Compare.ord a' b
-            {
-              apply And.intro
-              exact b_le_a
-              have : List.length as' + Nat.succ (List.length bs') < Nat.succ (List.length as') + Nat.succ (List.length bs') := by
-                apply Nat.add_lt_add_right
+            apply And.intro
+            exact Or.inr (Compare.flip h₀)
+            match bs' with
+            | [] => 
+              rw [empty_left]
+              rw [←Compare.ord_implies_eq h₀]
+              exact aas
+            | b''::bs'' =>
+              have : List.length as' + Nat.succ (List.length bs'') < Nat.succ (List.length as') + Nat.succ (Nat.succ (List.length bs'')) := by
+                apply Nat.add_lt_add <;>
                 apply Nat.lt_succ_self
-              have ⟨ _, right ⟩  := @list_sorted_nonempty α _ a' b as' (b'::bs') aas.right bbs
-              exact right (Or.inl h₀)
-            }
-            {
-              apply And.intro
+              have ⟨ _, right ⟩  := @list_sorted_nonempty α _ a' b' as' (b''::bs'') aas.right bbs.right
+              apply right
+              have : a = b' := Compare.ord_implies_eq h₀
+              rw [←this]
               exact aas.left
-              apply And.intro
-              exact Or.inr (Compare.flip h₀)
-              match as' with
-              | [] =>
-                rw [empty_right]
-                exact bbs
-              | a''::as'' =>
-                have : List.length as'' + Nat.succ (List.length bs') < Nat.succ (Nat.succ (List.length as'')) + Nat.succ (List.length bs') := by
-                  apply Nat.add_lt_add_right
-                  apply Nat.lt_trans (Nat.lt_succ_self _)
-                  apply Nat.lt_succ_self
-                have ⟨ _, right ⟩  := @list_sorted_nonempty α _ a'' b as'' (b'::bs') aas.right.right bbs
-                apply right
-                have : a' = b := Compare.ord_implies_eq h₀
-                rw [←this]
-                exact aas.right.left
-            }
-            {
-              apply And.intro
-              exact aas.left
-              have : List.length as' + Nat.succ (List.length bs') < Nat.succ (List.length as') + Nat.succ (List.length bs') := by
-                apply Nat.add_lt_add_right
-                apply Nat.lt_succ_self
-              have ⟨ left, _ ⟩  := @list_sorted_nonempty α _ a' b as' (b'::bs') aas.right bbs
-              exact left (Or.inl (Compare.flip h₀))
-            }
           }
           {
-            unfold List.concat_sorted
-            intro a_le_b
-            simp only
-            cases h₀:Compare.ord a b'
-            {
-              apply And.intro
-              exact bbs.left
-              have : Nat.succ (List.length as') + List.length bs' < Nat.succ (List.length as') + Nat.succ (List.length bs') := by
-                apply Nat.add_lt_add_left
-                apply Nat.lt_succ_self
-              have ⟨ _, right ⟩  := @list_sorted_nonempty α _ a b' (a'::as') bs' aas bbs.right
-              exact right (Or.inl h₀)
-            }
-            {
-              apply And.intro
-              exact a_le_b
-              apply And.intro
-              exact Or.inr (Compare.flip h₀)
-              match bs' with
-              | [] => 
-                rw [empty_left]
-                rw [←Compare.ord_implies_eq h₀]
-                exact aas
-              | b''::bs'' =>
-                have : List.length as' + Nat.succ (List.length bs'') < Nat.succ (List.length as') + Nat.succ (Nat.succ (List.length bs'')) := by
-                  apply Nat.add_lt_add <;>
-                  apply Nat.lt_succ_self
-                have ⟨ _, right ⟩  := @list_sorted_nonempty α _ a' b' as' (b''::bs'') aas.right bbs.right
-                apply right
-                have : a = b' := Compare.ord_implies_eq h₀
-                rw [←this]
-                exact aas.left
-            }
-            {
-              apply And.intro
-              exact a_le_b
-              have : Nat.succ (List.length as') + List.length bs' < Nat.succ (List.length as') + Nat.succ (List.length bs') := by
-                apply Nat.add_lt_add_left
-                apply Nat.lt_succ_self
-              have ⟨ left, _ ⟩  := @list_sorted_nonempty α _ a b' (a'::as') bs' aas bbs.right
-              exact left (Or.inl (Compare.flip h₀))
-            }
+            apply And.intro
+            exact a_le_b
+            have : Nat.succ (List.length as') + List.length bs' < Nat.succ (List.length as') + Nat.succ (List.length bs') := by
+              apply Nat.add_lt_add_left
+              apply Nat.lt_succ_self
+            have ⟨ left, _ ⟩  := @list_sorted_nonempty α _ a b' (a'::as') bs' aas bbs.right
+            exact left (Or.inl (Compare.flip h₀))
           }
-    termination_by _ => as.length + bs.length
-    decreasing_by {
-      simp_wf
-      try { assumption }
-      try { admit }
-    }
-  
-  theorem nonempty_left [Compare α] {{ a b: α }} (as bs : List α)
-      (aas: (a::as).sorted) (bbs : (b::bs).sorted) (b_le_a: b <= a):
-      List.sorted (a::List.concat_sorted as (b::bs)) := (list_sorted_nonempty  as bs aas bbs).left b_le_a
+        }
+  termination_by _ => as.length + bs.length
+  decreasing_by {
+    simp_wf
+    try { assumption }
+    try { admit }
+  }
 
-  theorem nonempty_right [Compare α] {{ a b: α }} (as bs : List α)
-      (aas: (a::as).sorted) (bbs : (b::bs).sorted)
-      (a_le_b: a <= b) : List.sorted (b::List.concat_sorted (a::as) bs) := (list_sorted_nonempty  as bs aas bbs).right a_le_b
+#print axioms concat_sorted.list_sorted_nonempty
 
-end concat_sorted
+theorem concat_sorted.nonempty_left [Compare α] {{ a b: α }} (as bs : List α)
+    (aas: (a::as).sorted) (bbs : (b::bs).sorted) (b_le_a: b <= a):
+    List.sorted (a::List.concat_sorted as (b::bs)) := (list_sorted_nonempty  as bs aas bbs).left b_le_a
+
+#print axioms concat_sorted.nonempty_left
+
+theorem concat_sorted.nonempty_right [Compare α] {{ a b: α }} (as bs : List α)
+    (aas: (a::as).sorted) (bbs : (b::bs).sorted)
+    (a_le_b: a <= b) : List.sorted (b::List.concat_sorted (a::as) bs) := (list_sorted_nonempty  as bs aas bbs).right a_le_b
+
+#print axioms concat_sorted.nonempty_right
 
 theorem concat_sorted.comm 
   [Compare α]
@@ -488,11 +529,11 @@ by
 
 #print axioms concat_sorted.keeps_sorted
 
-theorem concat_sorted_all [Compare α] {{P : α -> Prop}} :
+theorem concat_sorted.all [Compare α] {{P : α -> Prop}} :
   ∀{{alist blist: List α}},
   (alist.allP P) -> (blist.allP P) ->
   (alist.concat_sorted blist).allP P := by
-  apply List.concat_sorted.induction
+  apply concat_sorted.induction
   {
     intro bs _ all_bs
     rw [empty_right]
@@ -536,13 +577,13 @@ theorem concat_sorted_all [Compare α] {{P : α -> Prop}} :
     exact prev all_as.right all_bs
   }
 
-#print axioms concat_sorted_all 
+#print axioms concat_sorted.all 
 
-theorem concat_sorted_any [Compare α] {{P : α -> Prop}} :
+theorem concat_sorted.any [Compare α] {{P : α -> Prop}} :
   ∀{{alist blist: List α}},
   (alist.anyP P) ∨ (blist.anyP P) ->
   (alist.concat_sorted blist).anyP P := by
-  apply List.concat_sorted.induction
+  apply concat_sorted.induction
   {
     intro bs any_as_or_bs
     rw [empty_right]
@@ -589,4 +630,4 @@ theorem concat_sorted_any [Compare α] {{P : α -> Prop}} :
     | .inr any_bs => Or.inr (prev (Or.inr any_bs))
   }
 
-#print axioms concat_sorted_any
+#print axioms concat_sorted.any
